ctl_bind_af_l

theories/CTree/Logic/Trans.v
@@ -35,24 +35,23 @@ Section CTreeTrans.
   Context {E: Type} `{HE: Encode E} {X: Type}.
   Notation encode := (@encode E HE).
   
-  (* Note: This Kripke transition rel observes labels, this is important
-     for the [ktrans_bind_inv] lemma *)
+  (* The Kripke transition system *)
   Variant ktrans_: relation (ctree E X * World E) :=    
-    | KtransObs (ts: World E) (e: E) (x: encode e)
+    | KtransObs (w: World E) (e: E) (x: encode e)
         (t t': ctree E X):
       trans (obs e x) t t' ->
-      ~ is_done ts ->
-      ktrans_ (t, ts) (t', Obs e x)
-    | KtransTau (ts: World E) (t t': ctree E X):
+      not_done w ->
+      ktrans_ (t, w) (t', Obs e x)
+    | KtransTau (w: World E) (t t': ctree E X):
       trans tau t t' ->
-      ~ is_done ts ->
-      ktrans_ (t, ts) (t', ts)
-    | KtransRet (ts: World E) (t t': ctree E X) (x: X):
+      not_done w ->
+      ktrans_ (t, w) (t', w)
+    | KtransDone (x: X) (t t': ctree E X) w:
       trans (val x) t stuck ->
-      ~ is_done ts ->
       t' ≅ stuck ->
-      ktrans_ (t, ts) (t', Done x).
-
+      not_done w ->
+      ktrans_ (t, w) (t', Done x).
+  
   Global Instance trans_equ_proper:
     Proper (equ eq * eq ==> equ eq * eq ==> iff) ktrans_.
   Proof.
@@ -62,45 +61,42 @@ Section CTreeTrans.
     split; intros TR; inv TR.
     - apply KtransObs; auto. now rewrite <- Heqt0, <- Heqt. 
     - apply KtransTau; auto. now rewrite <- Heqt0, <- Heqt.
-    - apply KtransRet; auto.
+    - apply KtransDone; auto.
       + now rewrite <- Heqt.
-      + now rewrite <- Heqt0.                         
+      + now rewrite <- Heqt0.
     - apply KtransObs; auto. now rewrite Heqt0, Heqt.
     - apply KtransTau; auto. now rewrite Heqt0, Heqt.
-    - apply KtransRet; auto.
+    - apply KtransDone; auto.
       + now rewrite Heqt.
-      + now rewrite Heqt0. 
+      + now rewrite Heqt0.
   Qed.
-  
-  (*| This version is more amenable to induction |*)
+ 
+  (*| This version is more amenable to induction on [trans] |*)
   Lemma ktrans_trans: forall t t' w w',
       ktrans_ (t, w) (t', w') <->
         (exists l, trans_ l (observe t) (observe t') /\
-                ~ is_done w /\
+                not_done w /\
                 ((l = tau /\ w' = w)
                  \/ (exists e (x: encode e), l = obs e x /\ w' = Obs e x)
                  \/ (exists (x: X), l = val x /\ t' ≅ stuck /\ w' = Done x))).
   Proof.
-    intros; split; intro H.
-    inv H. 
-    - exists (obs e x); split; auto; split; auto.
-      right; left.
-      exists e, x; auto.
-    - exists tau; split; auto. 
-    - exists (val x); rewrite H6; split; auto; split; auto.
-      right; right.
-      exists x; auto.
-    - destruct H as (l & ? & ? & ?).
-      + destruct H1.
-        * destruct H1 as (-> & ->).
-          now apply KtransTau.
-        * destruct H1.
-          -- destruct H1 as (e & x & -> & ->).
-             now apply KtransObs.
-          -- destruct H1 as (x & -> & ? & ->).
-             rewrite H1 in *.
-             apply KtransRet; auto.
-  Qed.  
+    intros; split; intro H.    
+    - inv H. 
+      + exists (obs e x); split; auto; split; auto.
+        right; left.
+        exists e, x; auto.
+      + exists tau; split; auto.
+      + exists (val x); rewrite H5; split; auto; split; auto with ctl.
+        right; right.
+        exists x; auto.
+    - destruct H as (l & ? & ? & []).
+      + destruct H1 as (-> & ->).
+        now apply KtransTau.
+      + destruct H1 as [(e & x & -> & ->) | (x & -> & ? & ->)].
+        * now apply KtransObs.
+        * rewrite H1 in *.
+          apply KtransDone; auto with trans.
+  Qed.
 
 End CTreeTrans.
 
@@ -108,14 +104,13 @@ Ltac ktrans_inv H :=
   let Hw := fresh "Heqw" in
   let e := fresh "e" in
   let x := fresh "x" in
+  let v := fresh "v" in
   let l := fresh "l" in
-  let TR := fresh "TR" in
   let Ht := fresh "Heqt" in
   apply ktrans_trans in H as
-      (l & H & ? & [(Hl & Hw) | [(e & x & Hl & Hw) | (x & Hl & Ht & Hw)]]); subst.
-
-Ltac ktrans_goal :=
-  simpl ktrans; eexists; apply ktrans_trans.
+        (l & H & ? & [(Hl & Hw) |
+                        [(e & x & Hl & Hw) |
+                          (x & Hl & Ht & Hw) ]]); subst.
 
 Global Hint Constructors ktrans_: core.
 
@@ -127,24 +122,23 @@ Section CTreeTrans.
 
   (*| CTree is a kripke automaton with [Sb] equivalence |*)
   Global Program Instance ctree_kripke : Kripke (ctree E) sbisim E :=
-    {| ktrans X m m' := ktrans_ (X:=X) m m' |}.
+    {| ktrans X m m' := @ktrans_ E HE X m m' |}.
   Next Obligation.
     ktrans_inv H0;
       destruct (SBisim.sbisim_trans (X:=X) _ _ _ _ eq H H0)
-      as (l & c1' & ? & <- & ?).
-    + exists c1'; split; [apply KtransTau|]; auto.      
-    + exists c1'; split; [apply KtransObs|]; auto.
-    + exists c1'; split; auto.
+      as (l' & c1' & ? & <- & ?); exists c1'.
+    + split; [apply KtransTau|]; auto.      
+    + split; [apply KtransObs|]; auto.
+    + split; auto.
       pose proof trans_val_inv H2.
-      rewrite <- H4 in H2.
-      now apply KtransRet. 
+      rewrite <- H4 in *.
+      now apply KtransDone.
   Defined.
   Next Obligation.
-    ktrans_inv H; auto with ctl.
+    ktrans_inv H; auto with ctl; inv H0.
   Defined.
   Next Obligation.
-    intros (t' & w' & TR).
-    ktrans_inv TR; apply H; constructor. 
+    ktrans_inv H; apply H0; auto. 
   Defined.
 
   (*| Lemmas that depend on structure of [ctrees] |*)
@@ -159,7 +153,8 @@ Section CTreeTrans.
       + split; [eassumption|split]; auto.
         right; left; eauto.
       + split; [eassumption|split]; auto.
-        right; right; eauto.
+        right; right.
+        exists x; auto.
     - destruct H as (n' & H); ktrans_inv H; apply ktrans_trans; eexists.
       + split; [|split].
         * econstructor; eassumption.
@@ -172,12 +167,12 @@ Section CTreeTrans.
       + split; [|split].
         * econstructor; eassumption.
         * assumption.
-        * right; right; exists x; split; auto. 
+        * right; right; exists x; split; auto.
   Qed.
 
   Lemma ktrans_brS {X}: forall n (t: ctree E X) (k: fin' n -> ctree E X) w w',
       (BrS n k, w) ↦ (t, w') <->
-        (exists (i: fin' n), t ≅ k i /\ w = w' /\ ~ is_done w).
+        (exists (i: fin' n), t ≅ k i /\ w = w' /\ not_done w).
   Proof.
     split; intro H.
     - ktrans_inv H; apply trans_brS_inv in H as (n' & ? & ?);
@@ -198,18 +193,17 @@ Section CTreeTrans.
     - apply ktrans_brD; now (exists (F1)).
   Qed.
 
-  Lemma ktrans_ret {X}: forall (t: ctree E X) s s' x,
-      ktrans_ (Ret x, s) (t, s') <-> (s' = Done x /\ t ≅ stuck /\ ~ is_done s).
+  Lemma ktrans_ret {X}: forall (t: ctree E X) (w w': World E) (e: E) (v: encode e) x,
+      ktrans_ (Ret x, w) (t, w') <-> (not_done w /\ w' = Done x /\ t ≅ stuck).
   Proof.
     intros; split; intros.
-    - ktrans_inv H; dependent destruction H; auto.
-    - destruct H as (-> & -> & ?). 
-      apply KtransRet; etrans.
+    - ktrans_inv H; dependent destruction H; split; auto.
+    - destruct H as (? & -> & ->); etrans. 
   Qed.
 
   Lemma ktrans_vis{X}: forall (t: ctree E X) (s s': World E) (e: E) (k: encode e -> ctree E X),
       ktrans_ (Vis e k, s) (t, s') <->
-      (exists (x: encode e), s' = Obs e x /\ k x ≅ t /\ ~ is_done s).
+      (exists (x: encode e), s' = Obs e x /\ k x ≅ t /\ not_done s).
   Proof.
     intros; split; intro TR.
     - ktrans_inv TR.
@@ -226,25 +220,24 @@ Section CTreeTrans.
       right; left; eauto.
   Qed.
 
-  Lemma ktrans_not_started{X}: forall (t t': ctree E X) w,
-      ktrans_ (t, w) (t', NotStarted) ->
-        w = NotStarted.
+  Lemma ktrans_pure{X}: forall (t t': ctree E X) w,
+      ktrans_ (t, w) (t', Pure) -> w = Pure.
   Proof.
     intros * H.
     inv H; reflexivity.
   Qed.
-
+  Hint Resolve ktrans_pure: ctl.
+  
   Lemma ktrans_not_done{X}: forall (t t': ctree E X) w w',
-    (t, w) ↦ (t', w') ->
-    ~ is_done w.
+    (t, w) ↦ (t', w') -> not_done w.
   Proof.
-    intros; inv H; auto.
+    intros; inv H; auto with ctl.
   Qed.
   Hint Resolve ktrans_not_done: ctl.
             
   Lemma ktrans_bind_l{X Y}: forall (t t': ctree E Y) (k: Y -> ctree E X) w w',
       ktrans_ (t, w) (t', w') ->
-      ~ is_done w' ->
+      not_done w' ->
       ktrans_ (x <- t ;; k x, w) (x <- t' ;; k x, w').
   Proof.
     intros.
@@ -258,7 +251,7 @@ Section CTreeTrans.
         intro Hcontra; inv Hcontra; world_inv.
       + split; auto with ctl. (* Ret *)
         right; eauto.
-    - exfalso; apply H0; constructor. 
+    - inv H0.
   Qed.
 
   Lemma ktrans_bind_r{X Y}: forall (t: ctree E Y) (u: ctree E X) (k: Y -> ctree E X) (y: Y) w w',
@@ -267,12 +260,11 @@ Section CTreeTrans.
       ktrans_ (y <- t ;; k y, w) (u, w').
   Proof.
     intros.
-    ktrans_inv H; apply ktrans_trans.
-    - exfalso; apply H1; constructor.
-    - world_inv.
-    - ktrans_inv H0; world_inv.
+    ktrans_inv H; apply ktrans_trans; try world_inv.
+    - inv H1. 
+    - ktrans_inv H0. 
       + exists tau; split.
-        * apply trans_bind_r with x; etrans. 
+        * apply trans_bind_r with x; auto.          
         * split; auto.
       + exists (obs e x0); split.
         * apply trans_bind_r with x; etrans.
@@ -284,9 +276,10 @@ Section CTreeTrans.
           right; right; eauto.
   Qed.
 
-  Lemma ktrans_bind_inv{X Y}: forall (t: ctree E Y) (u: ctree E X) (k: Y -> ctree E X) w w',
+  Lemma ktrans_bind_inv{X Y}: forall (t: ctree E Y) (u: ctree E X) (k: Y -> ctree E X) (w w': @World E HE) ,
       ktrans_ (x <- t ;; k x, w) (u, w') ->
       (exists t', ktrans_ (t, w) (t', w')
+             /\ not_done w'
              /\ u ≅ x <- t' ;; k x) \/
       (exists y, ktrans_ (t, w) (stuck, Done y)
             /\ ktrans_ (k y, w) (u, w')).
@@ -294,37 +287,32 @@ Section CTreeTrans.
     intros * TR.
     ktrans_inv TR; destruct (trans_bind_inv _ _ TR) as
       [(Hv & t' & TR' & Heq) | (y & TRv & TR')]. 
-    + left; exists t'; split; auto.
-    + right; exists y; split; apply ktrans_trans.
-      * exists (val y); split; auto; split; auto with ctl.
-        right; right; exists y; auto.
-      * exists (tau); split; auto.
-    + left; exists t'; split; auto with ctl.
-    + right; exists y; cbn; auto with ctl.
-    + exfalso; apply Hv; constructor.
-    + right; exists y; cbn; split; auto.
-      apply ktrans_trans.
+    - left; exists t'; split; auto.
+    - right; exists y; split; auto; apply ktrans_trans.
+    - left; exists t'; split; auto with ctl.
+    - right; exists y; split; auto; apply ktrans_trans.
+    - exfalso; apply Hv; constructor.
+    - right; exists y; split; auto; apply ktrans_trans.
       exists (val x); split; [|split]; auto.
-      right; right; exists x; auto.
+      right; right.
+      exists x; auto.
   Qed.
 
 End CTreeTrans.
 
 Local Typeclasses Transparent equ.
-Lemma ktrans_trigger_inv `{ReSumRet E1 E2} {X}: forall (e: E2) w w' (k: encode (resum e) -> ctree E2 X) (u': ctree E2 X),
+Lemma ktrans_trigger_inv `{ReSumRet E1 E2}{X}:forall (e: E2) w w' (k: encode (resum e) -> ctree E2 X) (u': ctree E2 X),
       ktrans_ (z <- trigger e ;; k z, w) (u', w') ->
-      (exists z, w' = Obs e z /\ u' ≅ k z).
+      (not_done w /\ exists z, w' = Obs e z /\ u' ≅ k z).
 Proof.    
   intros.
   unfold trigger in H3.
-  destruct w'.
-  - rewrite bind_vis in H3.
-    apply ktrans_vis in H3 as (? & ? & ?); world_inv.
-  - apply ktrans_bind_inv in H3 as [(? & ? & ?) | (x0 & Hret & Hcont)].
-    + apply ktrans_vis in H3 as (y & ? & ? & ?).
-      unfold resum, ReSum_refl, resum_ret, ReSumRet_refl in *; world_inv.
-      exists y; setoid_rewrite <- H5 in H4; rewrite bind_ret_l in H4; auto.
-    + apply ktrans_vis in Hret as (? & ? & ?); world_inv. 
-  - rewrite bind_vis in H3.
-    apply ktrans_vis in H3 as (? & ? & ?); world_inv. 
+  apply ktrans_bind_inv in H3 as
+      [(t' & TR & Hd & Hequ) | (x & TR & Hequ)].
+  - apply ktrans_vis in TR as (y & ? & ? & ?).
+    unfold resum, ReSum_refl, resum_ret, ReSumRet_refl in *; world_inv.
+    split; [auto | exists y]; split; [reflexivity|].
+    now rewrite <- H4, bind_ret_l in Hequ.
+  - apply ktrans_vis in TR as (y & ? & ? & ?); world_inv.
 Qed.
+
